

forward:

- ①  $G = K K^T$   
 $A = I + \text{tril}(\text{diag}(b)G, -1)$
- ②  $B_K = \text{diag}(b)K, B_V = \text{diag}(b)V$
- ③  $W = A^T B_K, U = A^T B_V$
- ④  $X = U - W S^T$
- ⑤  $P = (Q K^T) \odot M$
- ⑥  $O = Q S^T + P X$
- ⑦  $S^+ = S + X^T K$

let  $\bar{x}$  be  $\frac{\partial L}{\partial x}$ , upstream  $\bar{S}^+, \bar{O}$

- ⑦  $\bar{S}^+ = \bar{S}^T, \bar{X}^+ = K(\bar{S}^+)^T, \bar{K}^+ = X \bar{S}^+$
- ⑥  $\bar{Q}^+ = \bar{O} S, \bar{S}^+ = \bar{O}^T Q$   
 $\bar{P}^+ = \bar{O} X^T, \bar{X}^+ = P^T \bar{O}$
- ⑤ let  $T = Q K^T \rightarrow \bar{T} = \bar{P} \odot M$   
 $\bar{Q}^+ = \bar{T} K, \bar{K}^+ = \bar{T}^T Q$
- ④  $\bar{U}^+ = \bar{X}, \bar{W}^+ = -\bar{X} S, \bar{S}^+ = -\bar{X}^T W$   
 $\bar{B}_K = A^{-T} \bar{W}, \bar{B}_V = A^{-T} \bar{U}$
- ③  $\bar{A}^+ = -A^{-T} \bar{W} W^T - A^{-T} \bar{U} U^T$

$$Y = A^T B \rightarrow AY = B$$

$$A(dY) + (dA)Y = dB$$

$$dY = -A^{-1}(dA)Y + A^{-1}dB$$

$$G := \frac{dL}{dY} \text{ By Riesz, } dL = \langle G, dY \rangle = \text{tr}(G^T dY)$$

$$dL = \text{tr}(G^T [-A^{-1}(dA)Y + A^{-1}dB])$$

$$= -\text{tr}(G^T A^{-1}(dA)Y) + \text{tr}(G^T A^{-1}dB)$$

$$\therefore \frac{dL}{dB} = A^T G \quad \rightarrow -\text{tr}((A^{-T}G)^T (dA)Y) = -\text{tr}(Y(A^{-T}G)^T (dA))$$

$$\frac{dL}{dA} = -A^T G Y^T = -\text{tr}((A^{-T}G Y^T)^T (dA))$$

$$\text{lower mask} = L_{rs} = \mathbf{1}[r > s]$$

$$A_{rs} = \delta_{rs} + L_{rs}(b_r G_{rs})$$

for A on diagonal or upper is constant so those  $\bar{b}$  &  $\bar{G} = 0$

$$r > s: A_{rs} = b_r G_{rs}$$

$$G = K K^T$$

$$dG = dK K^T + K dK^T$$

$$\bar{G} \cdot \frac{dL}{dG}$$

$$dL = \langle \bar{G}, dG \rangle$$

$$= \langle \bar{G}, dK K^T \rangle + \langle \bar{G}, K dK^T \rangle$$

$$= \langle \bar{G} K, dK \rangle + \langle \bar{G}^T K, dK \rangle$$

$$= \langle (\bar{G} + \bar{G}^T) K, dK \rangle$$

ess: trace is cyclic

$$B_K \in \mathbb{R}^{ex \times D} \quad (B_K)_{id} = b_i K_{id}$$

$$\bar{K}_{id}^+ = b_i (\bar{B}_K)_{id}$$

$$\bar{V}_{id}^+ = b_i (\bar{B}_V)_{id}$$

$$\bar{b}_i = \sum_{d=1}^D ((\bar{B}_K)_{id} K_{id} + (\bar{B}_V)_{id} V_{id})$$

$$\bar{b}_i = \sum_{s < i} \bar{A}_{is} G_{is}$$

$$\bar{G}_{is} = \bar{A}_{is} \frac{\partial A_{is}}{\partial G_{is}} = \begin{cases} \bar{A}_{is} b_i, i > s \\ 0, o/w \end{cases} = \text{tril}(\text{diag}(b) \bar{A}, -1)$$

$$\bar{K}^+ = (\bar{G} + \bar{G}^T) K$$

update  $\bar{S}^+ \leftarrow \bar{S}$ , then go previous chunk